sha/verif_sha_bdo2.v
@@ -17,7 +17,7 @@ Lemma sha256_block_data_order_return:
    LOCAL  (`(eq ctx) (eval_id _ctx))
    SEP 
    (`(array_at tuint Tsh (tuints (hash_block regs b)) 0 8 ctx);
-    K_vector;
+    `K_vector (eval_var _K256 (tarray tuint 64));
    `(array_at_ tuint Tsh 0 16) (eval_var _X (tarray tuint 16));
    `(data_block sh (intlist_to_Zlist b) data)))
   (Sreturn None)
@@ -26,7 +26,7 @@ Lemma sha256_block_data_order_return:
         (`(array_at tuint Tsh
              (tuints (hash_blocks init_registers (hashed ++ b))) 0 8 ctx) *
          `(data_block sh (intlist_to_Zlist b) data) *
-         K_vector))
+         `K_vector (eval_var _K256 (tarray tuint 64))))
      (stackframe_of f_sha256_block_data_order)).
 Proof.
 intros.
@@ -35,8 +35,7 @@ forward. (* return; *)
 unfold frame_ret_assert; simpl.
 unfold sha256state_.
 set (regs := hash_block (hash_blocks init_registers hashed) b).
-unfold K_vector; unfold_lift.
-erewrite elim_globals_only by (split3; [eassumption | reflexivity.. ]).
+unfold_lift.
 unfold stackframe_of; simpl.
 rewrite var_block_data_at_ by reflexivity.
 rewrite prop_true_andp by (compute; congruence).
